safety try 1

lemma/example_3.v
@@ -10,7 +10,8 @@ Definition prt_q:=1.
 Definition prt_r:=2.
 (*adopt the convention that all opts have the same length*)
 CoFixpoint T_p := ltt_send prt_q [Some (sint,T_p); Some (sint,ltt_end); None].
-CoFixpoint T_q := ltt_recv prt_p [Some (sint,T_q); Some (sint, ltt_send prt_r [None;None;Some (sint,ltt_end)]); None].
+Definition T_q1 :=ltt_send prt_r [None;None;Some (sint,ltt_end)].
+CoFixpoint T_q := ltt_recv prt_p [Some (sint,T_q); Some (sint, T_q1); None].
 Definition T_r := ltt_recv prt_q [None;None; Some (sint,ltt_end)].
 
 Definition gamma := M.add prt_p T_p (M.add prt_q T_q (M.add prt_r T_r M.empty)).
@@ -123,6 +124,10 @@ Qed.
 
 CoFixpoint inf_pq_path := cocons (gamma,(lcomm prt_p prt_q) 0) inf_pq_path.
 
+Ltac Mfind_normalise H0 := repeat (try rewrite M.add_spec1 in H0;
+try rewrite M.add_spec2 in H0; try rewrite M.remove_spec1 in H0;
+try rewrite M.remove_spec2 in H0; try rewrite M.empty_spec in H0; try easy).
+
 Theorem inf_pq_path_fair : fairness inf_pq_path.
 Proof.
     red.
@@ -140,22 +145,10 @@ Proof.
         apply lem_6_11c_tctx_comm_invert in H0.
         destr_hyps.
         destruct (Nat.eq_dec p prt_q);
-        destruct (Nat.eq_dec p prt_r); crush. 
-        unfold prt_r,prt_p,prt_q in *;crush.
+        destruct (Nat.eq_dec p prt_r); crush; 
+        unfold prt_r,prt_p,prt_q in *;crush;intros;Mfind_normalise H0;
 
-        intros.
-        unfold gamma in H0.
-        rewrite M.add_spec2 in H0.
-        rewrite M.add_spec1 in H0. rewrite (ltt_eq T_q) in H0. simpl in H0.
-        discriminate H0. crush.
-        
-        unfold gamma in H0.
-        rewrite M.add_spec2 in H0.
-        rewrite M.add_spec2 in H0.
-        rewrite M.add_spec1 in H0. rewrite (ltt_eq T_r) in H0. simpl in H0. discriminate. crush.
-        crush.
-        rewrite M.add_spec2 in H0; try rewrite M.add_spec2 in H0; try rewrite M.add_spec2 in H0;
-        try rewrite M.empty_spec in H0;crush.
+        rewrite (ltt_eq T_q) in H0;crush.
     }
     assert(H_q:q=prt_q).
     {
@@ -165,28 +158,15 @@ Proof.
         apply lem_6_11c_tctx_comm_invert in H0.
         destr_hyps.
         destruct (Nat.eq_dec q prt_p);
-        destruct (Nat.eq_dec q prt_r); crush.
-
-        unfold gamma in H0;
-        first rewrite M.add_spec2 in H0;
-        first rewrite M.add_spec2 in H0;
-        first rewrite M.add_spec2 in H0;
-        first rewrite M.empty_spec in H0;
-        first discriminate H0; crush.
-        
-        discriminate H0.
-        
-        unfold gamma in H1.
-        rewrite M.add_spec2 in H1.
-        rewrite M.add_spec2 in H1.
-        rewrite M.add_spec1 in H1. rewrite (ltt_eq T_r) in H1. simpl in H1. discriminate. crush.
-        crush.
-        rewrite M.add_spec2 in H1; try rewrite M.add_spec2 in H1; try rewrite M.add_spec2 in H1;
-        try rewrite M.empty_spec in H1;crush.
+        destruct (Nat.eq_dec q prt_r); crush;
+        unfold prt_r,prt_p,prt_q in *;crush;intros;Mfind_normalise H0.
+         rewrite (ltt_eq T_p) in H0;crush.
     }
     apply evh. subst. simpl. easy.
     right. assumption.
 Qed.
+
+
 
 Lemma red_5: tctxR gamma (lsend prt_p prt_q (Some sint) 1) (M.add prt_p ltt_end (M.add prt_q T_q (M.add prt_r T_r M.empty))).
 Proof.
@@ -210,63 +190,183 @@ Proof.
         - rewrite (ltt_eq T_q). apply Rrecv with (n:=1); try easy.
 Qed.
 
-Definition gamma' := M.add prt_p ltt_end (M.add prt_q (ltt_send prt_r [None;None;Some (sint,ltt_end)]) (M.add prt_r T_r M.empty)).
+Definition gamma' := M.add prt_p ltt_end (M.add prt_q T_q1 (M.add prt_r T_r M.empty)).
+
+Definition m_update2 p q Tp Tq (gamma:tctx) := 
+    M.add p Tp (M.add q Tq (M.remove p (M.remove q gamma))).
+
 
 Lemma red_7 : tctxR gamma (lcomm prt_p prt_q 1) gamma'.
 Proof.
-    set (p_only := M.add prt_p T_p M.empty).
-    set (q_only := M.add prt_q T_q M.empty).
-    
-    set (p_only' := M.add prt_p ltt_end M.empty).
-    set (q_only' := M.add prt_q (ltt_send prt_r [None;None;Some (sint,ltt_end)]) M.empty).
-    assert(Hp1: tctxR p_only (lsend prt_p prt_q (Some sint) 1) p_only').
+    Search "simple" "red".
+    assert ( M.Equal (M.add prt_p ltt_end (M.add prt_q T_q1 (M.remove prt_p (M.remove prt_q gamma)))) gamma').
     {
-        unfold p_only.
-        unfold p_only'.
-        rewrite (ltt_eq T_p).
-        apply Rsend with (n:=1); try easy.   
+        unfold M.Equal;intros.
+        unfold gamma'.
+        destruct (Nat.eq_dec y prt_p);   
+        destruct (Nat.eq_dec y prt_q);crush.
     }
-    assert(Hq1: tctxR q_only (lrecv prt_q prt_p (Some sint) 1) q_only').
-    {
-        unfold q_only.
-        unfold q_only'.
-        rewrite (ltt_eq T_q).
-        apply Rrecv with (n:=1); try easy.   
-    }
-    assert(H_disj:MF.Disjoint p_only q_only).
-    {
-        unfold MF.Disjoint. unfold not.
-        intros.
-        destruct H.
-        apply MF.add_in_iff in H.
-        destruct H.
-        {
-            subst. apply MF.in_find in H0.
-            unfold M.find in H0. simpl in H0. easy.
-        }
-        {
-            apply MF.not_in_empty in H. assumption.
-        }
-    }
+    setoid_rewrite <- H.
+    eapply simple_red_comm with (sp:=sint) (sq:=sint);try easy.
 
-    set (pq := M.add prt_p T_p (M.add prt_q T_q M.empty)).
-    set (pq' := M.add prt_p ltt_end (M.add prt_q (ltt_send prt_r [None;None;Some (sint, ltt_end)]) M.empty)).
+    unfold gamma.
+    rewrite M.add_spec1. rewrite (ltt_eq T_p). simpl. reflexivity.
+    rewrite M.add_spec2;try rewrite M.add_spec1; try rewrite (ltt_eq T_q);
+    try easy; reflexivity.
+    1-2:crush. apply srefl. 
+Qed.
+
+Lemma red_8 : tctxR gamma' (lsend prt_q prt_r (Some sint) 2) (m_update prt_q ltt_end gamma').
+Proof.
+    unfold gamma', prt_q, prt_r;
+    eapply simple_red_send;crush.
+Qed. 
+
+Lemma red_9 : tctxR gamma' (lrecv prt_r prt_q (Some sint) 2) (m_update prt_r ltt_end gamma').
+Proof.
+    unfold gamma', prt_q, prt_r;
+    eapply simple_red_recv;crush.
+Qed.
+
+Definition gamma_end := M.add prt_p ltt_end (M.add prt_q ltt_end (M.add prt_r ltt_end M.empty)).
+
+Lemma red_10 : tctxR gamma' (lcomm prt_q prt_r 2) gamma_end.
+Proof.
+    assert (M.Equal (m_update2 prt_q prt_r ltt_end ltt_end gamma') gamma_end).
+    {
+        unfold gamma';red;intros.
+        destruct (Nat.eq_dec y prt_q);   
+        destruct (Nat.eq_dec y prt_r); crush.
+    }
+    setoid_rewrite <- H.
+    unfold prt_q, prt_r; eapply simple_red_comm;crush;apply srefl.
+Qed.
+Print coseq.
+Definition label_dc := (lcomm 0 0 0).
+
+Lemma gamma_possible_comm: forall p q k gamma2, tctxR gamma (lcomm p q k) gamma2 ->
+    (p=prt_p /\ q=prt_q /\ k =0) \/ (p=prt_p /\ q=prt_q /\ k = 1).
+Proof.
+    intros.
+    eapply lem_6_11c_tctx_comm_invert in H. destr_hyps.
+    rename x into s1, x0 into s2, x1 into xp, x3 into xq,x4 into Tq, x2 into Tp.
+    destruct (Nat.eq_dec prt_p p);destruct (Nat.eq_dec prt_q q);crush.
+    {
+        unfold gamma in H. Mfind_normalise H. rewrite (ltt_eq T_p) in H. simpl in H.
+        inversion H;subst.
+        destruct (Nat.eq_dec k 0);   
+        destruct (Nat.eq_dec k 1);crush.
+        assert  (exists n, k=S (S n)).
+        {
+            destruct k;crush. destruct k;crush. exists k. easy.
+        }
+        destruct H6 as [k' Hk'].
+        rewrite Hk' in H4. simpl in H4.
+        destruct k';crush.
+        rewrite onth_nil in H4;easy.
+    }
+    {
+        destruct (Nat.eq_dec q prt_p);
+        destruct (Nat.eq_dec q prt_r);
+        unfold gamma in H0;Mfind_normalise H0;unfold prt_p, prt_r in *;crush;
+        unfold gamma in H; Mfind_normalise H; inversion H;
+        rewrite (ltt_eq T_p) in H7; simpl in H7; inversion H7.
+    }
+    {
+         destruct (Nat.eq_dec p prt_q);
+        destruct (Nat.eq_dec p prt_r);
+        unfold prt_p, prt_r in *;crush;
+        unfold gamma in H; Mfind_normalise H; inversion H;
+        rewrite (ltt_eq T_p) in H7; simpl in H7; inversion H7. 
+    }
+    {
+           destruct (Nat.eq_dec p prt_q);
+        destruct (Nat.eq_dec p prt_r);
+        unfold prt_p, prt_q, prt_r in *;crush;
+        unfold gamma in H; Mfind_normalise H; inversion H;
+        rewrite (ltt_eq T_q) in H7; simpl in H7; inversion H7. 
+    }
+Qed.
+Lemma gamma'_possible_comm : forall q r k gamma2, tctxR gamma' (lcomm q r k) gamma2 ->
+    (q=prt_q /\ r =prt_r /\ k = 2 ).
+Proof.
+    intros.
+    eapply lem_6_11c_tctx_comm_invert in H. destr_hyps.
+    rename x into s1, x0 into s2, x1 into xp, x3 into xq,x4 into Tq, x2 into Tp.
     
-    assert(H_eqn: M.Equal (disj_merge p_only q_only H_disj) (M.add prt_p T_p (M.add prt_q T_q M.empty))).
+    destruct (Nat.eq_dec q prt_q);destruct (Nat.eq_dec r prt_r);subst.
     {
-        unfold M.Equal.
-        intros.
-        unfold disj_merge.
-        rewrite MF.merge_spec1mn; try easy.
-        unfold p_only. unfold q_only.
-        do 4 rewrite MF.add_o.
-        Search M.find M.empty.
-        rewrite M.empty_spec.
-        destruct (Nat.eq_dec prt_p y); destruct (Nat.eq_dec prt_q y); try (simpl; easy).
-        subst. discriminate.
+        unfold gamma' in H. Mfind_normalise H.
+        rewrite (ltt_eq T_q1) in H. simpl in H. inversion H;subst.
+        destruct k. 
+        simpl in H4;crush.
+        destruct k. 
+        simpl in H4;crush.
+        destruct k;try easy.
+        simpl in H4;rewrite onth_nil in H4; crush.
     }
-    assert (Hpq : tctxR pq (lcomm prt_p prt_q 1) pq').
     {
-     unfold pq. unfold pq'. admit.
+        destruct (Nat.eq_dec r prt_p);
+        destruct (Nat.eq_dec r prt_q);
+        unfold gamma in H0;Mfind_normalise H0;unfold prt_p, prt_r in *;crush;
+        unfold gamma in H; Mfind_normalise H; inversion H;
+        rewrite (ltt_eq T_p) in H7; simpl in H7; inversion H7.
     }
-Abort.
+    {
+         destruct (Nat.eq_dec q prt_p);
+        destruct (Nat.eq_dec q prt_r);
+        unfold prt_p, prt_r in *;crush;
+        unfold gamma in H; Mfind_normalise H;crush. 
+    }
+    {
+        destruct (Nat.eq_dec q prt_p);
+        destruct (Nat.eq_dec q prt_r);
+        unfold prt_p, prt_r in *;crush;
+        unfold gamma in H; Mfind_normalise H;crush.
+    }
+Qed.
+
+Lemma gamma_end_possible_comm: forall p q k gamma2, tctxR gamma_end (lcomm p q k) gamma2 ->
+    False.
+Proof.
+    intros.
+    eapply lem_6_11c_tctx_comm_invert in H. destr_hyps.
+    rename x into s1, x0 into s2, x1 into xp, x3 into xq,x4 into Tq, x2 into Tp.
+    unfold gamma_end in *.
+    destruct (Nat.eq_dec p prt_p);
+    destruct (Nat.eq_dec p prt_q);
+    destruct (Nat.eq_dec p prt_r);
+    unfold prt_p, prt_q, prt_r;crush;Mfind_normalise H;crush.
+Qed.
+Lemma gamma_weak_safe: weak_safety gamma.
+Proof.
+Admitted.
+Lemma gamma'_weak_safe: weak_safety gamma'.
+Proof.
+Admitted.
+Lemma gamma_end_weak_safe: weak_safety gamma_end.
+Proof. Admitted.
+Lemma gamma_safe: safeC gamma.
+Proof.
+    Check safety_red.
+    pcofix CIH.
+    pfold.
+    constructor; try apply gamma_weak_safe.
+    intros.
+    pose proof H as Hred.
+    eapply gamma_possible_comm in H.
+    destruct H.
+    {
+        destr_hyps;subst.
+        pose proof red_3 as Hrk.
+        pose proof Hred as Hred2.
+        eapply lem_6_12_reduction_determinism with (g':= gamma) in Hred;try easy.
+        split. eapply weak_safe_meq_invariant with (c:=gamma);try easy; try apply gamma_weak_safe.
+        left.
+    }
+Admitted.
+Definition path_0 := cocons (gamma, (lcomm prt_p prt_q 0)) 
+    (cocons (gamma, (lcomm prt_p prt_q 1)) 
+        (cocons (gamma', (lcomm prt_q prt_r 2)) 
+            (cocons (gamma_end, label_dc) conil))
+    ).
