src/path_props.v
@@ -1,6 +1,6 @@
 (* From mathcomp Require Import ssreflect.seq all_ssreflect. *)
 From Paco Require Import paco pacotac.
-From SST Require Import src.expr src.header src.local src.lcontext.
+From SST Require Import src.expr src.header src.local src.lcontext CpdtTactics.
 Require Import List String Coq.Arith.PeanoNat Morphisms Relations.
 Require Import Coq.Program.Equality.
 Import ListNotations.
@@ -46,45 +46,21 @@ Definition enabled (F: tctx -> Prop) (pt: Path): Prop :=
 
 Definition headRecv (p q: part) (pt: Path): Prop :=
   match pt with
-    | cocons (g, (lrecv a b (Some s) n)) xs => if andb (Nat.eqb p a) (Nat.eqb q b) then True else False
+    | cocons (g, (lrecv a b (Some s) n)) xs => if Nat.eq_dec p a then if Nat.eq_dec q b then True else False else False
     | _                                   => False 
   end.
 
 Definition headSend (p q: part) (pt: Path): Prop :=
   match pt with
-    | cocons (g, (lsend a b (Some s) n)) xs => if andb (Nat.eqb p a) (Nat.eqb q b) then True else False
+    | cocons (g, (lsend a b (Some s) n)) xs => if Nat.eq_dec p a then if Nat.eq_dec q b then True else False else False
     | _                                   => False 
   end.
 
 Definition headComm (p q: part) (pt: Path): Prop :=
   match pt with
-    | cocons (g, (lcomm a b n)) xs => if andb (Nat.eqb p a) (Nat.eqb q b) then True else False
+    | cocons (g, (lcomm a b n)) xs => if Nat.eq_dec p a then if Nat.eq_dec q b then True else False else False
     | _                          => False 
   end.
-
-Inductive immTrans: part -> part -> Path -> Prop :=
-  | immTc: forall p q c pt n, immTrans p q (cocons (c,(lcomm p q n)) pt).
-
-Lemma eqvL: forall p q pt, immTrans p q pt -> headComm p q pt.
-Proof. intros. induction H. cbn. rewrite !Nat.eqb_refl. easy. Qed.
-
-Lemma eqvR: forall p q pt, headComm p q pt -> immTrans p q pt.
-Proof. intros.
-       destruct pt. simpl in H. easy.
-       simpl in H.
-       destruct p0, l.
-       easy.
-       easy.
-       case_eq((p =? n)); intros.
-       + rewrite Nat.eqb_eq in H0.
-         subst.
-         case_eq((q =? n0)); intros.
-         ++ rewrite Nat.eqb_eq in H0.
-            subst.
-            constructor.
-         ++ rewrite H0 in H. rewrite Nat.eqb_refl in H. simpl in H. easy.
-       + rewrite H0 in H. simpl in H. easy.
-Qed.
 
 Definition fairPath (pt: Path): Prop :=
   forall p q n, enabled (tctxRE (lcomm p q n)) pt ->  eventually (headComm p q) pt.
@@ -95,6 +71,80 @@ Definition livePath (pt: Path) : Prop := forall p q s n,
 enabled (tctxRE (lsend p q (Some s) n)) pt -> eventually (headComm p q) pt /\
 enabled (tctxRE (lrecv p q (Some s) n)) pt -> eventually (headComm p q) pt.
 Definition liveness := alwaysC livePath.
+
+Definition weak_safety (c: tctx ) :=
+forall p q s s'  k k', tctxRE (lsend p q (Some s) k) c -> tctxRE (lrecv q p (Some s') k') c ->
+                               tctxRE (lcomm p q k) c.
+
+Inductive safe (R: tctx -> Prop): tctx -> Prop :=
+  | safety_red :  forall c, weak_safety c -> (forall p q c' k, 
+    tctxR c (lcomm p q k) c' -> (weak_safety c' /\ (forall c'', M.Equal c c'' -> R c''))) 
+    -> safe R c.
+                               (*
+Definition weak_safe_tctx := {c | weak_safety c}.
+Inductive safe (R: weak_safe_tctx -> Prop): weak_safe_tctx -> Prop :=
+  | safety_red :  forall c, (forall p q c' k, 
+    tctxR (proj1_sig c) (lcomm p q k) c' -> (exists P, R (exist weak_safety c' P))) 
+    -> safe R c.
+*)
+Definition safeC c := paco1 safe bot1 c.
+
+Lemma safe_monotone : monotone1 safe.
+Proof.
+  unfold monotone1.
+  intros.
+  induction IN. 
+  eapply safety_red with (c:=c) ;try easy.
+  intros.
+  eapply H0 in H1. destr_hyps. split; try easy.
+  intros. eapply LE. eapply H2. easy. 
+Qed.
+
+#[global] Instance RWMTCTXR: Proper ((@M.Equal ltt) ==> (eq) ==> (@M.Equal ltt) ==> (iff)) tctxR.
+Proof. unfold "==>". constructor; intros; subst. 
+apply Rstruct with (g1:=y) (g2:=y1) (g1':=x) (g2':=x1);crush. 
+apply Rstruct with (g1:=x) (g2:=x1) (g1':=y) (g2':=y1);crush.
+Qed.
+Lemma weak_safe_meq_invariant: forall c c', weak_safety c -> M.Equal c c' -> 
+  weak_safety c'.
+Proof.
+  intros.
+  unfold weak_safety.
+  intros.
+  unfold weak_safety in H.
+  unfold tctxRE in *. destr_hyps. rename x0 into g1, x into g2. 
+  specialize (H p q s s' k k'). setoid_rewrite <- H0 in H1.
+  setoid_rewrite <- H0 in H2.
+  setoid_rewrite <- H0.
+  apply H;[exists g1 | exists g2];easy. 
+Qed.
+
+Lemma safe_meq_invariant: forall c c', safeC c -> M.Equal c c' -> safeC c'.
+Proof.
+  intros.
+  pcofix CIH.
+  pfold. constructor.
+  { 
+    pinversion H;try apply safe_monotone. 
+    eapply weak_safe_meq_invariant with (c':=c') in H1; try easy. 
+  }
+  {
+    intros.
+    pinversion H;try apply safe_monotone;subst. setoid_rewrite <- H0 in H1.
+    pose proof H1 as Htx.
+    eapply H3 in H1.
+    split;try easy.
+
+    destr_hyps.
+    intros.
+    setoid_rewrite H5 in H0. 
+    eapply H4 in H0.
+    destruct H0;crush.
+    Search paco1 bot1. 
+    left.
+    eapply paco1_mon_bot with (gf:=safe); try easy.
+  } 
+Qed.
 (*
 Inductive livePath (pt: Path): Prop :=
   | L1: forall p q s, enabled (tctxRE (lsend p q (Some s) n)) pt -> eventually (headComm p q) pt -> livePath pt
